8th homework

sf/Assignment08_02.v
@@ -9,16 +9,45 @@ Require Export Assignment08_01.
    (this latter part is trickier than you might expect). *)
 
 Definition pup_to_n : com :=
-  FILL_IN_HERE.
+  Y ::= (ANum 0) ;;
+  WHILE BNot (BEq (AId X) (ANum 0)) DO
+    Y ::= (APlus (AId Y) (AId X));;
+    X ::= (AMinus (AId X) (ANum 1))
+  END.
 
 Example pup_to_2_ceval :
   pup_to_n / (update empty_state X 2) ||
     update (update (update (update (update (update empty_state
       X 2) Y 0) Y 2) X 1) Y 3) X 0.
 Proof.
-  exact FILL_IN_HERE.
+unfold pup_to_n.
+  eapply E_Seq with (st':=(update (update empty_state X 2) Y 0)).
+  eapply E_Ass.
+  reflexivity.
+  eapply E_WhileLoop with (st':=(update (update (update (update empty_state X 2) Y 0) Y 2) X 1)).
+  reflexivity.
+  eapply E_Seq with (st':=(update (update (update empty_state X 2) Y 0) Y 2)).
+  eapply E_Ass.
+  compute.
+  reflexivity.
+  eapply E_Ass.
+  compute.
+  reflexivity.
+  eapply E_WhileLoop with (st':= update (update (update (update (update (update empty_state X 2) Y 0) Y 2) X 1)
+        Y 3) X 0).
+  simpl.
+  reflexivity.
+  eapply E_Seq with (st':= (update (update (update (update (update empty_state X 2) Y 0) Y 2) X 1) Y 3)).
+  eapply E_Ass.
+  simpl.
+  reflexivity.
+  eapply E_Ass.
+  simpl.
+  reflexivity.
+  eapply E_WhileEnd.
+  simpl.
+  reflexivity.
 Qed.
-
 (*-- Check --*)
 Check pup_to_2_ceval :
   pup_to_n / (update empty_state X 2) ||
