sf/Assignment08_05.v
@@ -7,7 +7,13 @@ Require Export Assignment08_04.
     same as pushing the value of the expression on the stack. *)
 
 Fixpoint s_compile (e : aexp) : list sinstr :=
-  FILL_IN_HERE.
+match e with
+    | ANum n => [ SPush n ]
+    | AId ident => [ SLoad ident ]
+    | APlus e1 e2 => (s_compile e1) ++ (s_compile e2) ++ [ SPlus ]
+    | AMinus e1 e2 => (s_compile e1) ++ (s_compile e2) ++ [ SMinus ]
+    | AMult e1 e2 => (s_compile e1) ++ (s_compile e2) ++ [ SMult ]
+  end.
 
 (** After you've defined [s_compile], prove the following to test
     that it works. *)
@@ -16,7 +22,8 @@ Example s_compile1 :
     s_compile (AMinus (AId X) (AMult (ANum 2) (AId Y)))
   = [SLoad X; SPush 2; SLoad Y; SMult; SMinus].
 Proof.
-  exact FILL_IN_HERE.
+  simpl.
+  reflexivity.
 Qed.
 
 (** **** Exercise: 3 stars, advanced (stack_compiler_correct)  *)
@@ -33,10 +40,111 @@ Qed.
     general lemma to get a usable induction hypothesis; the main
     theorem will then be a simple corollary of this lemma. *)
 
+Theorem execute_theorem : forall (e : aexp) (st : state) (s1 : list nat) (other : list sinstr),
+		s_execute st s1 (s_compile e ++ other) =
+				s_execute st ((aeval st e) :: s1) other.
+Proof.
+induction e; try reflexivity.
+simpl in |- *.
+intros st s1 other.
+assert
+((s_compile e1 ++ s_compile e2 ++ [SPlus]) ++ other =
+ s_compile e1 ++ s_compile e2 ++ [SPlus] ++ other).
+rewrite -> app_ass.
+rewrite -> app_ass.
+reflexivity.
+
+rewrite H in |- *.
+assert
+(s_execute st s1 (s_compile e1 ++ s_compile e2 ++ SPlus :: other) =
+ s_execute st (aeval st e1 :: s1) (s_compile e2 ++ SPlus :: other)).
+apply IHe1.
+
+simpl in |- *.
+rewrite H0 in |- *.
+assert
+(s_execute st (aeval st e1 :: s1) (s_compile e2 ++ SPlus :: other) =
+ s_execute st (aeval st e2 :: aeval st e1 :: s1) (SPlus :: other)).
+apply IHe2.
+
+rewrite H1 in |- *.
+simpl in |- *.
+rewrite plus_comm in |- *.
+reflexivity.
+
+intros st s1 other.
+assert
+(s_execute st s1 (s_compile e1 ++ s_compile e2 ++ SMinus :: other) =
+ s_execute st (aeval st e1 :: s1) (s_compile e2 ++ SMinus :: other)).
+apply IHe1.
+
+simpl in |- *.
+assert
+((s_compile e1 ++ s_compile e2 ++ [SMinus]) ++ other =
+ s_compile e1 ++ s_compile e2 ++ [SMinus] ++ other).
+rewrite -> app_ass.
+rewrite -> app_ass.
+reflexivity.
+
+simpl in |- *.
+rewrite H0 in |- *.
+simpl in |- *.
+rewrite H in |- *.
+assert
+(s_execute st (aeval st e1 :: s1) (s_compile e2 ++ SMinus :: other) =
+ s_execute st (aeval st e2 :: aeval st e1 :: s1) (SMinus :: other)).
+apply IHe2.
+
+rewrite H1 in |- *.
+simpl in |- *.
+reflexivity.
+
+intros st s1 other.
+simpl in |- *.
+simpl in |- *.
+assert
+((s_compile e1 ++ s_compile e2 ++ [SMult]) ++ other =
+ s_compile e1 ++ s_compile e2 ++ [SMult] ++ other).
+rewrite -> app_ass.
+rewrite -> app_ass.
+reflexivity.
+
+rewrite H in |- *.
+simpl in |- *.
+assert
+(s_execute st s1 (s_compile e1 ++ s_compile e2 ++ SMult :: other) =
+ s_execute st (aeval st e1 :: s1) (s_compile e2 ++ SMult :: other)).
+apply IHe1.
+
+rewrite H0 in |- *.
+assert
+(s_execute st (aeval st e1 :: s1) (s_compile e2 ++ SMult :: other) =
+ s_execute st (aeval st e2 :: aeval st e1 :: s1) (SMult :: other)).
+apply IHe2.
+
+rewrite H1 in |- *.
+simpl in |- *.
+rewrite mult_comm in |- *.
+reflexivity.
+Qed.
+
+
 Theorem s_compile_correct : forall (st : state) (e : aexp),
   s_execute st [] (s_compile e) = [ aeval st e ].
 Proof.
-  exact FILL_IN_HERE.
+intros st e.
+assert ([aeval st e] = s_execute st [aeval st e] []).
+simpl in |- *.
+reflexivity.
+
+rewrite H in |- *.
+assert (s_compile e ++ [] = s_compile e).
+simpl in |- *.
+rewrite -> app_nil_end.
+reflexivity.
+
+rewrite <- H0 in |- *.
+apply execute_theorem.
 Qed.
 
 (*-- Check --*)
