sf/Assignment08_04.v
@@ -8,16 +8,63 @@ Require Export Assignment08_03.
 
 (* Hint *)
 Check andb_true_iff.
-
 Theorem no_whiles_terminate: forall c st
     (NOWHL: no_whiles c = true),
   exists st', c / st || st'.
 Proof.
-  exact FILL_IN_HERE.
+  intros.
+  generalize dependent st.
+  induction c.
+  intros.
+  exists st.
+  apply E_Skip.
+  intros.
+  exists (update st i (aeval st a)).
+  apply E_Ass.
+  reflexivity.
+  intros.
+  inversion NOWHL.
+  subst.
+  assert (exists st', c1 / st || st') as term_fst.
+  apply IHc1. 
+  apply andb_true_iff in H0.
+  inversion H0.
+  apply H.
+  inversion term_fst.
+  assert (exists st'', c2 / x || st'') as term_snd.
+  apply IHc2. 
+  apply andb_true_iff in H0.
+  inversion H0.
+  apply H2.
+  inversion term_snd.
+  exists x0.
+  apply E_Seq with x; assumption.
+  intros.
+  inversion NOWHL.
+  subst.
+  assert (exists st', c1 / st || st') as term_then.
+  apply IHc1.
+  apply andb_true_iff in H0.
+  inversion H0.
+  apply H.
+  inversion term_then.
+  assert (exists st', c2 / st || st') as term_else.
+  apply IHc2.
+  apply andb_true_iff in H0.
+  inversion H0.
+  apply H2.
+  inversion term_else.
+  remember (beval st b) as evalb.
+  destruct evalb.
+  exists x.
+  apply E_IfTrue. symmetry. assumption. assumption.
+  exists x0.
+  apply E_IfFalse. symmetry. assumption. assumption.
+  inversion NOWHL.
 Qed.
-
 (*-- Check --*)
 Check no_whiles_terminate: forall c st
     (NOWHL: no_whiles c = true),
   exists st', c / st || st'.
+
 
