sf/Assignment08_07.v
@@ -9,7 +9,19 @@ Theorem IFB_false: forall b c1 c2,
     (IFB b THEN c1 ELSE c2 FI) 
     c2.
 Proof.
-  exact FILL_IN_HERE.
+  intros.
+  unfold cequiv.
+  split.
+  intros.
+  inversion H0.
+  subst.
+  unfold bequiv in H.
+  simpl in H.
+  rewrite H in H6.
+  inversion H6.
+  assumption.
+  eapply E_IfFalse.
+  eapply H.
 Qed.
 
 (*-- Check --*)
