sf/Assignment08_09.v
@@ -11,8 +11,34 @@ Theorem WHILE_true: forall b c,
      cequiv 
        (WHILE b DO c END)
        (WHILE BTrue DO SKIP END).
-Proof. 
-  exact FILL_IN_HERE.
+Proof.
+  intros.
+  split.
+  intros.
+Lemma WHILE_true_nonterm : forall b c st st',
+     bequiv b BTrue ->
+     ~( (WHILE b DO c END) / st || st' ).
+Proof.
+  intros b c st st' Hb.
+  intros H.
+  remember (WHILE b DO c END) as cw.
+  ceval_cases (induction H) Case;
+  inversion Heqcw; subst; clear Heqcw.
+  unfold bequiv in Hb.
+  rewrite Hb in H. inversion H.
+  apply IHceval2. reflexivity.
+Qed.
+  apply WHILE_true_nonterm in H0.
+  apply ex_falso_quodlibet.
+  assumption.
+  assumption.
+  intros.
+  apply WHILE_true_nonterm in H0.
+  apply ex_falso_quodlibet.
+  assumption.
+  unfold bequiv.
+  simpl.
+  reflexivity.
 Qed.
 
 (*-- Check --*)
