sf/Assignment08_10.v
@@ -6,7 +6,24 @@ Require Export Assignment08_09.
 Theorem seq_assoc : forall c1 c2 c3,
   cequiv ((c1;;c2);;c3) (c1;;(c2;;c3)).
 Proof.
-  exact FILL_IN_HERE.
+  intros.
+  split.
+  intros.
+  inversion H; subst.
+  inversion H2; subst.
+  econstructor.
+  eapply H3.
+  eapply E_Seq.
+  eapply H7.
+  eapply H5.
+  intros.
+  inversion H; subst.
+  inversion H5; subst.
+  eapply E_Seq.
+  eapply E_Seq.
+  eapply H2.
+  eapply H3.
+  eapply H7.
 Qed.
 
 (*-- Check --*)
