sf/Assignment08_11.v
@@ -7,7 +7,36 @@ Theorem assign_aequiv : forall X e,
   aequiv (AId X) e -> 
   cequiv SKIP (X ::= e).
 Proof.
-  exact FILL_IN_HERE.
+  Lemma update_same : forall n1 x1 x2 (st : state), st x1 = n1 -> (update st x1 n1) x2 = st x2.
+  Proof.
+    intros.
+    unfold update.
+    destruct (eq_id_dec x1 x2).
+    symmetry.
+    rewrite <- e.
+    eapply H.
+    reflexivity.
+  Qed.
+
+  intros.
+  split; intros; inversion H0; subst.
+  assert (st' = update st' X (aeval st' e)).
+  apply functional_extensionality.
+  intro.
+  rewrite update_same.
+  reflexivity.
+  apply H.
+  rewrite -> H1 at 2.
+  eapply E_Ass.
+  reflexivity.
+  assert (st = update st X (aeval st e)).
+  apply functional_extensionality.
+  intro.
+  rewrite update_same.
+  reflexivity.
+  apply H.
+  rewrite <- H1.
+  constructor.
 Qed.
 
 (*-- Check --*)
