sf/Assignment08_12.v
@@ -6,8 +6,23 @@ Require Export Assignment08_11.
 Theorem CSeq_congruence : forall c1 c1' c2 c2',
   cequiv c1 c1' -> cequiv c2 c2' ->
   cequiv (c1;;c2) (c1';;c2').
-Proof. 
-  exact FILL_IN_HERE.
+Proof.
+  intros.
+  split.
+  intros.
+  inversion H1; subst.
+  eapply E_Seq.
+  eapply H.
+  eapply H4.
+  eapply H0.
+  eapply H7.
+  intros.
+  inversion H1; subst.
+  eapply E_Seq.
+  eapply H.
+  eapply H4.
+  eapply H0.
+  eapply H7.
 Qed.
 
 (*-- Check --*)
@@ -15,3 +30,5 @@ Check CSeq_congruence : forall c1 c1' c2 c2',
   cequiv c1 c1' -> cequiv c2 c2' ->
   cequiv (c1;;c2) (c1';;c2').
 
+
+  
