sf/Assignment08_13.v
@@ -7,7 +7,32 @@ Theorem CIf_congruence : forall b b' c1 c1' c2 c2',
   bequiv b b' -> cequiv c1 c1' -> cequiv c2 c2' ->
   cequiv (IFB b THEN c1 ELSE c2 FI) (IFB b' THEN c1' ELSE c2' FI).
 Proof.
-  exact FILL_IN_HERE.
+  intros.
+  split.
+  intros.
+  inversion H2; subst.
+  eapply E_IfTrue.
+  rewrite <- H.
+  eapply H8.
+  eapply H0.
+  eapply H9.
+  eapply E_IfFalse.
+  rewrite <- H.
+  eapply H8.
+  eapply H1.
+  eapply H9.
+  intros.
+  inversion H2; subst.
+  eapply E_IfTrue.
+  rewrite <- H in H8.
+  eapply H8.
+  eapply H0 in H9.
+  eapply H9.
+  eapply E_IfFalse.
+  rewrite <- H in H8.
+  eapply H8.
+  eapply H1 in H9.
+  eapply H9.
 Qed.
 
 (*-- Check --*)
