sf/Assignment08_17.v
@@ -5,7 +5,28 @@ Require Export Assignment08_16.
 Lemma optimize_0plus_bexp_sound:
   btrans_sound optimize_0plus_bexp.
 Proof.
-  exact FILL_IN_HERE.
+  unfold btrans_sound.
+  intros.
+  unfold bequiv.
+  intros.
+  induction b.
+  simpl.
+  reflexivity.
+  simpl.
+  reflexivity.
+  simpl.
+  rewrite <- 2 optimize_0plus_aexp_sound.
+  reflexivity.
+  simpl.
+  rewrite <- 2 optimize_0plus_aexp_sound.
+  reflexivity.
+  simpl.
+  rewrite IHb.
+  reflexivity.
+  simpl.
+  rewrite IHb1.
+  rewrite IHb2.
+  reflexivity.
 Qed.
 
 (*-- Check --*)
