sf/Assignment08_18.v
@@ -4,10 +4,30 @@ Require Export Assignment08_17.
 
 Lemma optimize_0plus_com_sound:
   ctrans_sound optimize_0plus_com.
-Proof.
-  exact FILL_IN_HERE.
+Proof. unfold ctrans_sound. intros c. unfold cequiv.
+  com_cases (induction c) Case.
+  reflexivity.
+  apply CAss_congruence.
+  apply optimize_0plus_aexp_sound.
+  simpl.
+  apply CSeq_congruence.
+  unfold cequiv.
+  apply IHc1.
+  unfold cequiv.
+  apply IHc2.
+  simpl.
+  apply CIf_congruence.
+  apply optimize_0plus_bexp_sound.
+  unfold cequiv.
+  apply IHc1.
+  unfold cequiv.
+  apply IHc2.
+  simpl.
+  apply CWhile_congruence.
+  apply optimize_0plus_bexp_sound.
+  unfold cequiv.
+  apply IHc.
 Qed.
-
 (*-- Check --*)
 Check optimize_0plus_com_sound:
   ctrans_sound optimize_0plus_com.
