sf/Assignment08_19.v
@@ -1,11 +1,18 @@
 Require Export Assignment08_18.
 
 (* problem #19: 10 points *)
-
 Lemma constfold_0plus_sound:
   ctrans_sound constfold_0plus.
 Proof.
-  exact FILL_IN_HERE.
+  unfold constfold_0plus.
+  simpl.
+  unfold ctrans_sound.
+  intros c.
+  remember (fold_constants_com c).
+  apply trans_cequiv with c0.
+  rewrite Heqc0.
+  apply fold_constants_com_sound.
+  apply optimize_0plus_com_sound. 
 Qed.
 
 (*-- Check --*)
