sf/Prop.v
@@ -2,6 +2,8 @@
 
 Require Export Logic.
 
+Require Export Basics.
+
 (* ####################################################### *)
 (** * Inductively Defined Propositions *)
 
